

Bài 9 x

$$a) (P \wedge Q) \rightarrow P$$

$$= \bar{P} \vee \bar{Q} \vee P = \bar{Q} \vee 1 = 1$$

$$b) P \rightarrow (\bar{P} \rightarrow P)$$

$$= \bar{P} \vee (P \vee P) = 1 \vee P = 1$$

$$c) P \rightarrow ((Q \rightarrow (P \wedge Q)))$$

$$= \bar{P} \vee ((\bar{Q} \vee (P \wedge Q))) = \bar{P} \vee (\bar{Q} \vee P) = \bar{Q} \vee 1 = 1$$

$$d) \overline{P \vee \bar{Q}} \rightarrow \bar{P}$$

$$= \bar{P} \vee \bar{Q} \vee \bar{P} = \bar{Q} \vee 1 = 1$$

Thấy 4 mệnh đề trên là hằng đúng

$$e) ((P \rightarrow Q) \wedge (Q \rightarrow R)) \rightarrow (P \rightarrow R)$$

$$= (P \wedge \bar{Q}) \vee (Q \wedge \bar{R}) \vee \bar{P} \vee R$$

$$= (\bar{P} \vee \bar{Q}) \vee (R \vee Q) = \bar{P} \vee R \vee (\bar{Q} \vee Q) = 1$$

Bài 10

$$\begin{aligned} a) \quad F \rightarrow G &= [P \wedge (Q \vee R)] \rightarrow [(P \wedge Q) \vee R] \\ &= [\bar{P} \vee \overline{(Q \vee R)}] \vee [(P \wedge Q) \vee R] \\ &= \bar{P} \vee [(\overline{Q \vee R}) \vee [(R \vee P) \wedge (R \vee Q)]] \\ &= \bar{P} \vee [(\overline{Q \vee R}) \vee (R \vee P)] \\ &= \bar{P} \vee [(\overline{Q \vee R}) \vee R \vee P] \\ &= \bar{P} \vee (\overline{Q \vee R}) \vee R \vee P \Leftrightarrow (\overline{Q \vee R}) \vee R \vee 1 \\ &= 1 \end{aligned}$$

Thấy $F \rightarrow G = 1$.

$$\begin{aligned}
 \text{b) } F \rightarrow G &= [(P \rightarrow Q) \wedge (Q \rightarrow R)] \rightarrow [P \rightarrow (Q \rightarrow R)] \\
 &= [\overline{(P \rightarrow Q)} \vee \overline{(Q \rightarrow R)}] \vee [\bar{P} \vee (\bar{Q} \vee R)] \\
 &= (\bar{P} \vee Q) \vee (\bar{Q} \vee R) \vee \bar{P} \vee \bar{Q} \vee R \\
 &= (P \wedge \bar{Q}) \vee (Q \wedge \bar{R}) \vee \bar{P} \vee \bar{Q} \vee R \\
 &= [(P \wedge \bar{Q}) \vee \bar{P}] \vee [(Q \wedge \bar{R}) \vee R] \vee \bar{Q} \\
 &= [(P \wedge \bar{Q}) \vee \bar{P}] \vee 1 = 1
 \end{aligned}$$

Vậy $F \rightarrow G = 1$ (G là hệ quả của F).

$$\begin{aligned}
 \text{c) } F \rightarrow G &= (P \wedge Q) \rightarrow [(P \rightarrow Q) \vee (P \rightarrow \bar{Q})] \\
 &= \overline{(P \wedge Q)} \vee [(P \vee Q) \vee (P \vee \bar{Q})] \\
 &= \bar{P} \vee \bar{Q} \vee P \vee Q \vee \bar{P} \vee \bar{Q} \\
 &= (\bar{P} \vee P) \vee (\bar{Q} \vee Q) \vee \bar{P} \vee \bar{Q} \\
 &= 1 \vee 1 \vee \bar{P} \vee \bar{Q} = 1
 \end{aligned}$$

Vậy $F \rightarrow G = 1$.

Bài 11

$$\begin{aligned}
 \text{a) } (P \vee Q) \wedge \overline{P \wedge Q} &\Leftrightarrow P \\
 &\Leftrightarrow (P \vee Q) \wedge (P \vee \bar{Q}) \Leftrightarrow P \\
 &\Leftrightarrow P \vee (Q \wedge \bar{Q}) \Leftrightarrow P \\
 &\Leftrightarrow P \vee 0 \Leftrightarrow P \\
 &\Leftrightarrow P \Leftrightarrow P
 \end{aligned}$$

$$b) \overline{(P \vee Q) \wedge R \vee \bar{Q}} \Leftrightarrow Q \wedge R$$

$$\Leftrightarrow (P \vee Q) \wedge R \wedge Q \Leftrightarrow Q \wedge R$$

$$\Leftrightarrow ((P \vee Q) \wedge Q) \wedge R \Leftrightarrow Q \wedge R$$

$$\Leftrightarrow Q \wedge R \Leftrightarrow Q \wedge R$$

$$c) ((P \vee Q) \wedge (P \vee \bar{Q})) \vee Q \Leftrightarrow P \vee Q$$

$$\Leftrightarrow (P \vee (Q \wedge \bar{Q})) \vee Q \Leftrightarrow P \vee Q$$

$$\Leftrightarrow P \vee Q \Leftrightarrow P \vee Q$$

$$d) \overline{P \vee Q} \vee ((\bar{P} \wedge Q) \vee \bar{Q}) \Leftrightarrow \overline{Q \wedge P}$$

$$\Leftrightarrow (\bar{P} \wedge \bar{Q}) \vee ((\bar{P} \vee \bar{Q}) \wedge (Q \vee \bar{Q})) \Leftrightarrow \overline{Q \wedge P}$$

$$\Leftrightarrow (\bar{P} \wedge \bar{Q}) \vee (\bar{P} \vee \bar{Q}) \Leftrightarrow \overline{Q \wedge P}$$

$$\Leftrightarrow \overline{(\bar{P} \vee \bar{P}) \wedge (\bar{P} \vee \bar{Q})} \vee \bar{Q}$$

$$\Leftrightarrow \bar{P} \wedge \bar{Q} \Leftrightarrow [(\bar{P} \wedge \bar{Q}) \vee \bar{P}] \vee \bar{Q} \Leftrightarrow \overline{Q \wedge P}$$

$$\Leftrightarrow \bar{P} \vee \bar{Q} \Leftrightarrow \overline{Q \wedge P}$$

$$\Leftrightarrow P \wedge Q \Leftrightarrow \overline{Q \wedge P}$$

$$e) (P \rightarrow Q) \wedge (\bar{Q} \wedge (R \vee \bar{Q})) \Leftrightarrow \overline{Q \vee P}$$

$$\Leftrightarrow (\bar{P} \vee Q) \wedge \bar{Q} \wedge (R \vee \bar{Q}) \Leftrightarrow \overline{Q \vee P}$$

$$\Leftrightarrow (\bar{P} \wedge \bar{Q}) \wedge (R \vee \bar{Q}) \Leftrightarrow \overline{Q \vee P}$$

$$\Leftrightarrow \bar{P} \wedge [\bar{Q} \wedge (R \vee \bar{Q})] \Leftrightarrow \overline{Q \vee P}$$

$$\Leftrightarrow \bar{P} \wedge \bar{Q} \Leftrightarrow \overline{Q \vee P}$$

$$\Leftrightarrow P \vee Q \Leftrightarrow \overline{Q \vee P}$$

$$f) P \vee (P \wedge (P \vee Q)) \Leftrightarrow P.$$

$$\Leftrightarrow P \vee P \Leftrightarrow P \Leftrightarrow P \Leftrightarrow P$$

$$g) P \vee Q \vee (\bar{P} \wedge \bar{Q} \wedge R) \Leftrightarrow P \vee Q \vee R.$$

$$\Leftrightarrow P \vee (Q \vee (\bar{P} \wedge \bar{Q} \wedge R)) \Leftrightarrow P \vee Q \vee R$$

$$\Leftrightarrow P \vee ((Q \vee \bar{P}) \wedge (Q \vee \bar{Q}) \wedge (Q \vee R)) \Leftrightarrow P \vee Q \vee R.$$

$$\Leftrightarrow P \vee ((Q \vee \bar{P}) \wedge (Q \vee R)) \Leftrightarrow P \vee Q \vee R$$

$$\Leftrightarrow (Q \vee \bar{P} \vee P) \wedge (Q \vee R \vee P) \Leftrightarrow P \vee Q \vee R$$

$$\Leftrightarrow (Q \vee 1) \wedge (Q \vee R \vee P) \Leftrightarrow P \vee Q \vee R$$

$$\Leftrightarrow Q \vee R \vee P \Leftrightarrow P \vee Q \vee R$$

$$h) (\bar{P} \vee \bar{Q}) \rightarrow (P \wedge Q \wedge R) \Leftrightarrow P \wedge Q.$$

$$\Leftrightarrow (P \wedge Q) \vee ((P \wedge Q) \wedge R) \Leftrightarrow P \wedge Q.$$

$$\Leftrightarrow P \wedge Q \Leftrightarrow P \wedge Q.$$

$$i) P \wedge ((\bar{Q} \rightarrow (R \wedge R)) \vee Q \vee (R \wedge S) \vee (R \wedge \bar{S})) \Leftrightarrow P$$

$$\Leftrightarrow P \wedge (Q \vee R \vee (\bar{Q} \wedge (R \wedge S) \wedge (R \wedge \bar{S}))) \Leftrightarrow P.$$

$$\Leftrightarrow P \wedge (Q \vee R \vee (\bar{Q} \wedge (\bar{R} \vee \bar{S}) \wedge (\bar{R} \vee S))) \Leftrightarrow P.$$

$$\Leftrightarrow P \wedge (Q \vee R \vee (\bar{Q} \wedge (\bar{R} \vee (\bar{S} \wedge S)))) \Leftrightarrow P$$

$$\Leftrightarrow P \wedge (Q \vee R \vee (\bar{Q} \wedge \bar{R})) \Leftrightarrow P$$

$$\Leftrightarrow P \wedge (Q \vee (R \vee \bar{Q})) \Leftrightarrow P$$

$$\Leftrightarrow P \wedge (Q \vee \bar{Q} \vee R) \Leftrightarrow P \Leftrightarrow P \Leftrightarrow P.$$

$$j) (P \vee Q \vee R) \wedge (P \vee S \vee \bar{Q}) \wedge (P \vee \bar{S} \vee R) \Leftrightarrow P \vee (R \wedge (S \vee \bar{Q}))$$

$$\text{Ga co } \Leftrightarrow P \vee ((Q \vee R) \wedge (S \vee \bar{Q}) \wedge (\bar{S} \vee R))$$

$$= P \vee ((R \vee (Q \wedge \bar{S})) \wedge (S \vee \bar{Q}))$$

$$= P \vee (R \wedge (S \vee \bar{Q})) = VP.$$